% Equation 1
\begin{dmath}
\exp\left({c}\right)^{\left(-{\sigma}\right)}=\exp\left({c}\right)^{\left(-{\sigma}\right)}\, \frac{{\beta}}{{\gamma_x}}\, \left({\alpha}\, \exp\left({z}\right)\, \left(\frac{\exp\left({k}\right)}{\exp\left({l}\right)}\right)^{{\alpha}-1}+1-{\delta}\right)
\end{dmath}
% Equation 2
\begin{dmath}
\frac{{\psi}\, \exp\left({c}\right)^{{\sigma}}}{1-\exp\left({l}\right)}=\exp\left({w}\right)
\end{dmath}
% Equation 3
\begin{dmath}
{\gamma_x}\, \exp\left({k}\right)=\exp\left({k}\right)\, \left(1-{\delta}\right)+\exp\left({{i}}\right)
\end{dmath}
% Equation 4
\begin{dmath}
\exp\left({y}\right)=\exp\left({c}\right)+\exp\left({{i}}\right)
\end{dmath}
% Equation 5
\begin{dmath}
\exp\left({y}\right)=\exp\left({z}\right)\, \exp\left({k}\right)^{{\alpha}}\, \exp\left({l}\right)^{1-{\alpha}}
\end{dmath}
% Equation 6
\begin{dmath}
\exp\left({w}\right)=\frac{\exp\left({y}\right)\, \left(1-{\alpha}\right)}{\exp\left({l}\right)}
\end{dmath}
% Equation 7
\begin{dmath}
{r}=\frac{\exp\left({y}\right)\, {\alpha}\, 4}{\exp\left({k}\right)}
\end{dmath}
% Equation 8
\begin{dmath}
{z}={z}\, {\rho_z}+{{\varepsilon_z^{surprise}}}+{{\varepsilon_z^{news}}}
\end{dmath}
% Equation 9
\begin{dmath}
{AUX\_EXO\_LAG\_8\_0}={{\varepsilon_z^{news}}}
\end{dmath}
% Equation 10
\begin{dmath}
{AUX\_EXO\_LAG\_8\_1}={{\varepsilon_z^{news}}}
\end{dmath}
% Equation 11
\begin{dmath}
{AUX\_EXO\_LAG\_8\_2}={{\varepsilon_z^{news}}}
\end{dmath}
% Equation 12
\begin{dmath}
{AUX\_EXO\_LAG\_8\_3}={{\varepsilon_z^{news}}}
\end{dmath}
% Equation 13
\begin{dmath}
{AUX\_EXO\_LAG\_8\_4}={{\varepsilon_z^{news}}}
\end{dmath}
% Equation 14
\begin{dmath}
{AUX\_EXO\_LAG\_8\_5}={{\varepsilon_z^{news}}}
\end{dmath}
% Equation 15
\begin{dmath}
{AUX\_EXO\_LAG\_8\_6}={{\varepsilon_z^{news}}}
\end{dmath}
% Equation 16
\begin{dmath}
{AUX\_EXO\_LAG\_8\_7}={{\varepsilon_z^{news}}}
\end{dmath}
